{
 "cells": [
  {
   "cell_type": "markdown",
   "id": "1708c832",
   "metadata": {},
   "source": [
    "# ðŸ“˜ Derivative of the Sigmoid Function\n",
    "\n",
    "---\n",
    "\n",
    "## ðŸ§  Definition of Sigmoid Function\n",
    "\n",
    "The sigmoid (logistic) function is defined as:\n",
    "\n",
    "```math\n",
    "Ïƒ(x) = \\frac{1}{1 + e^{-x}}\n",
    "```\n",
    "\n",
    "It maps any real number to the range (0, 1).\n",
    "\n",
    "---\n",
    "\n",
    "## ðŸŽ¯ Goal\n",
    "\n",
    "Find the derivative:\n",
    "\n",
    "```math\n",
    "\\frac{dÏƒ(x)}{dx}\n",
    "```\n",
    "\n",
    "---\n",
    "\n",
    "## ðŸ”„ Step-by-Step Derivation\n",
    "\n",
    "### Step 1: Rewrite Ïƒ(x) for differentiation\n",
    "\n",
    "Let:\n",
    "\n",
    "```math\n",
    "Ïƒ(x) = y = \\frac{1}{1 + e^{-x}}\n",
    "```\n",
    "\n",
    "Differentiate y with respect to x:\n",
    "\n",
    "```math\n",
    "\\frac{dy}{dx} = \\frac{d}{dx} \\left[\\frac{1}{1 + e^{-x}}\\right]\n",
    "```\n",
    "\n",
    "---\n",
    "\n",
    "### Step 2: Use the chain rule and quotient rule\n",
    "\n",
    "Let:\n",
    "\n",
    "* `u(x) = 1`\n",
    "* `v(x) = 1 + e^{-x}`\n",
    "\n",
    "Then using the quotient rule:\n",
    "\n",
    "```math\n",
    "\\frac{dy}{dx} = \\frac{v \\cdot \\frac{du}{dx} - u \\cdot \\frac{dv}{dx}}{v^2}\n",
    "```\n",
    "\n",
    "Since:\n",
    "\n",
    "* `du/dx = 0`\n",
    "* `dv/dx = -e^{-x}`\n",
    "\n",
    "We get:\n",
    "\n",
    "```math\n",
    "\\frac{dy}{dx} = \\frac{0 - (1)(-e^{-x})}{(1 + e^{-x})^2} = \\frac{e^{-x}}{(1 + e^{-x})^2}\n",
    "```\n",
    "\n",
    "---\n",
    "\n",
    "### Step 3: Express in terms of Ïƒ(x)\n",
    "\n",
    "Recall:\n",
    "\n",
    "```math\n",
    "Ïƒ(x) = \\frac{1}{1 + e^{-x}} \\Rightarrow 1 - Ïƒ(x) = \\frac{e^{-x}}{1 + e^{-x}}\n",
    "```\n",
    "\n",
    "Now multiply:\n",
    "\n",
    "```math\n",
    "Ïƒ(x) (1 - Ïƒ(x)) = \\left(\\frac{1}{1 + e^{-x}}\\right) \\left(\\frac{e^{-x}}{1 + e^{-x}}\\right) = \\frac{e^{-x}}{(1 + e^{-x})^2}\n",
    "```\n",
    "\n",
    "Which matches our earlier result.\n",
    "\n",
    "---\n",
    "\n",
    "## âœ… Final Result\n",
    "\n",
    "```math\n",
    "\\frac{dÏƒ(x)}{dx} = Ïƒ(x)(1 - Ïƒ(x))\n",
    "```\n",
    "\n",
    "---\n",
    "\n",
    "## ðŸ§ª Example\n",
    "\n",
    "If `x = 0`:\n",
    "\n",
    "```math\n",
    "Ïƒ(0) = \\frac{1}{1 + 1} = 0.5 \\\\\n",
    "\\frac{dÏƒ(0)}{dx} = 0.5(1 - 0.5) = 0.25\n",
    "```\n",
    "\n",
    "---\n",
    "\n",
    "## ðŸ“Œ Summary\n",
    "\n",
    "* The sigmoid derivative is compact and elegant.\n",
    "* It only depends on the output of the sigmoid itself.\n",
    "* Very efficient in neural network backpropagation.\n"
   ]
  },
  {
   "cell_type": "markdown",
   "id": "09d14dcb",
   "metadata": {},
   "source": []
  }
 ],
 "metadata": {
  "language_info": {
   "name": "python"
  }
 },
 "nbformat": 4,
 "nbformat_minor": 5
}
